Refactor and consolidate LowStar.Buffer
- LowStar.Modifies merged into LowStar.Buffer
- disjoint <==> loc_disjoint
- includes <==> loc_includes and (both null or both not null)
- two disjoint buffers, at least one of size nonzero, are distinct

ulib/LowStar.Buffer.fsti
@@ -196,59 +196,6 @@ let get (#a: Type) (h: HS.mem) (p: buffer a) (i: nat) : Ghost a
 = Seq.index (as_seq h p) i
 
 
-/// A buffer ``smaller`` is included in another buffer ``larger``, denoted
-/// as ``includes larger smaller``, if ``smaller`` is a sub-buffer of
-/// ``larger``. (See ``gsub`` below for how to actually construct such a
-/// sub-buffer of a buffer.)
-
-val includes (#a: Type) (larger smaller: buffer a) : GTot Type0
-
-
-/// The liveness of a sub-buffer is exactly equivalent to the liveness
-/// of its enclosing buffer.
-
-val includes_live (#a: Type) (h: HS.mem) (larger smaller: buffer a) : Lemma
-  (requires (larger `includes` smaller))
-  (ensures (live h larger <==> live h smaller))
-  [SMTPatOr [
-    [SMTPat (includes larger smaller); SMTPat (live h larger)];
-    [SMTPat (includes larger smaller); SMTPat (live h smaller)];
-  ]]
-
-
-/// If the contents of a buffer are equal in two given heaps, then so
-/// are the contents of any of its sub-buffers.
-
-val includes_as_seq (#a: Type) (h1 h2: HS.mem) (larger smaller: buffer a) : Lemma
-  (requires (larger `includes` smaller /\ as_seq h1 larger == as_seq h2 larger))
-  (ensures (as_seq h1 smaller == as_seq h2 smaller))
-
-
-/// Inclusion is a preorder.
-
-val includes_refl (#a: Type) (x: buffer a) : Lemma
-  (includes x x)
-  [SMTPat (includes x x)]
-
-val includes_trans (#a: Type) (x y z: buffer a) : Lemma
-  (requires (x `includes` y /\ y `includes` z))
-  (ensures (x `includes` z))
-  [SMTPatOr [
-    [SMTPat (x `includes` y); SMTPat (y `includes` z)];
-    [SMTPat (x `includes` y); SMTPat (x `includes` z)];
-    [SMTPat (y `includes` z); SMTPat (x `includes` z)];
-  ]]
-
-
-/// A buffer and any of its sub-buffers live in the same region, and
-/// at the same address, and are either both null or both not null.
-
-val includes_frameOf_as_addr (#a: Type) (larger smaller: buffer a) : Lemma
-  (requires (larger `includes` smaller))
-  (ensures (g_is_null larger == g_is_null smaller /\ frameOf larger == frameOf smaller /\ as_addr larger == as_addr smaller))
-  [SMTPat (larger `includes` smaller)]
-
-
 /// ``gsub`` is the way to carve a sub-buffer out of a given
 /// buffer. ``gsub b i len`` return the sub-buffer of ``b`` starting from
 /// offset ``i`` within ``b``, and with length ``len``. Of course ``i`` and
@@ -261,6 +208,8 @@ val gsub (#a: Type) (b: buffer a) (i: U32.t) (len: U32.t) : Ghost (buffer a)
   (requires (U32.v i + U32.v len <= length b))
   (ensures (fun y -> True))
 
+// goffset
+
 /// A buffer is live exactly at the same time as all of its sub-buffers.
 
 val live_gsub (#a: Type) (h: HS.mem) (b: buffer a) (i: U32.t) (len: U32.t) : Lemma
@@ -268,14 +217,10 @@ val live_gsub (#a: Type) (h: HS.mem) (b: buffer a) (i: U32.t) (len: U32.t) : Lem
   (ensures (live h (gsub b i len) <==> live h b))
   [SMTPat (live h (gsub b i len))]
 
-
-/// A sub-buffer is included in its enclosing buffer.
-
-val includes_gsub (#a: Type) (b: buffer a) (i: U32.t) (len: U32.t) : Lemma
+val gsub_is_null (#t: Type) (b: buffer t) (i: U32.t) (len: U32.t) : Lemma
   (requires (U32.v i + U32.v len <= length b))
-  (ensures (b `includes` gsub b i len))
-  [SMTPat (gsub b i len)]
-
+  (ensures (g_is_null (gsub b i len) <==> g_is_null b))
+  [SMTPat (g_is_null (gsub b i len))]
 
 /// The length of a sub-buffer is exactly the one provided at ``gsub``.
 
@@ -315,79 +260,1254 @@ val as_seq_gsub (#a: Type) (h: HS.mem) (b: buffer a) (i: U32.t) (len: U32.t) : L
   [SMTPat (as_seq h (gsub b i len))]
 
 
-/// Two buffers are disjoint only if they span disjoint ranges of a
-/// common enclosing buffer, or if they live in different regions or
-/// at different addresses.
+/// # The modifies clause
+///
+/// The modifies clause for regions, references and buffers.
+/// ==========================================================
+///
+/// This module presents the modifies clause, a way to track the set
+/// of memory locations modified by a stateful Low* (or even F*)
+/// program. The basic principle of modifies clauses is that any
+/// location that is disjoint from a set of memory locations modified
+/// by an operation is preserved by that operation.
+///
+/// We start by specifying a monoid of sets of memory locations. From
+/// a rough high-level view, ``loc`` is the type of sets of memory
+/// locations, equipped with an identity element ``loc_none``,
+/// representing the empty set, and an associative and commutative
+/// operator, ``loc_union``, representing the union of two sets of
+/// memory locations.
+///
+/// Moreover, ``loc_union`` is idempotent, which is useful to cut SMT
+/// matching loops with ``modifies_trans`` and ``modifies_refl`` below.
 
-val disjoint (#a1 #a2: Type) (b1: buffer a1) (b2: buffer a2) : GTot Type0
+val loc : Type0
+
+val loc_none: loc
+
+val loc_union
+  (s1 s2: loc)
+: GTot loc
+
+val loc_union_idem
+  (s: loc)
+: Lemma
+  (loc_union s s == s)
+  [SMTPat (loc_union s s)]
+
+val loc_union_comm
+  (s1 s2: loc)
+: Lemma
+  (loc_union s1 s2 == loc_union s2 s1)
+  [SMTPat (loc_union s1 s2)]
+
+val loc_union_assoc
+  (s1 s2 s3: loc)
+: Lemma
+  (loc_union s1 (loc_union s2 s3) == loc_union (loc_union s1 s2) s3)
+
+let loc_union_idem_1
+  (s1 s2: loc)
+: Lemma
+  (loc_union s1 (loc_union s1 s2) == loc_union s1 s2)
+  [SMTPat (loc_union s1 (loc_union s1 s2) == loc_union s1 s2)]
+= loc_union_assoc s1 s1 s2
+
+let loc_union_idem_2
+  (s1 s2: loc)
+: Lemma
+  (loc_union (loc_union s1 s2) s2 == loc_union s1 s2)
+  [SMTPat (loc_union (loc_union s1 s2) s2)]
+= loc_union_assoc s1 s2 s2
+
+val loc_union_loc_none_l
+  (s: loc)
+: Lemma
+  (loc_union loc_none s == s)
+  [SMTPat (loc_union loc_none s)]
+
+val loc_union_loc_none_r
+  (s: loc)
+: Lemma
+  (loc_union s loc_none == s)
+  [SMTPat (loc_union s loc_none)]
 
 
-/// Disjointness is symmetric.
+/// ``loc_buffer b`` is the set of memory locations associated to a buffer ``b``.
 
-val disjoint_sym (#a1 #a2: Type) (b1: buffer a1) (b2: buffer a2) : Lemma
-  (disjoint b1 b2 <==> disjoint b2 b1)
-  [SMTPat (disjoint b1 b2)]
+val loc_buffer
+  (#t: Type)
+  (b: buffer t)
+: GTot loc
 
-
-/// If two buffers are disjoint, then so are any of their sub-buffers.
-
-val disjoint_includes_l (#a1 #a2: Type) (b1 b1' : buffer a1) (b2: buffer a2) : Lemma
-  (requires (includes b1 b1' /\ disjoint b1 b2))
-  (ensures (disjoint b1' b2))
-  [SMTPat (disjoint b1' b2); SMTPat (includes b1 b1')] 
-
-val disjoint_includes_r (#a1 #a2: Type) (b1 : buffer a1) (b2 b2': buffer a2) : Lemma
-  (requires (includes b2 b2' /\ disjoint b1 b2))
-  (ensures (disjoint b1 b2'))
-  [SMTPat (disjoint b1 b2'); SMTPat (includes b2 b2')] 
+val loc_buffer_null
+  (t: Type)
+: Lemma
+  (loc_buffer (null #t) == loc_none)
+  [SMTPat (loc_buffer (null #t))]
 
 
-/// A buffer that has not been allocated yet is disjoint from all
-/// buffers that are already currently allocated. Consequently, two
-/// buffers that are allocated separately are disjoint.
+/// ``loc_addresses r n`` is the set of memory locations associated to a
+/// set of addresses ``n`` in a given region ``r``.
 
-val live_unused_in_disjoint (#a1 #a2: Type) (h: HS.mem) (b1: buffer a1) (b2: buffer a2) : Lemma
-  (requires (live h b1 /\ (unused_in b2 h)))
-  (ensures (disjoint b1 b2))
-(*
-  [SMTPatOr [
-    [SMTPat (live h b1); SMTPat (disjoint b1 b2)];
-    [SMTPat (live h b1); SMTPat (unused_in b2 h)];
-    [SMTPat (unused_in b2 h); SMTPat (disjoint b1 b2)];
-  ]]
-*)
+val loc_addresses
+  (preserve_liveness: bool)
+  (r: HS.rid)
+  (n: Set.set nat)
+: GTot loc
 
-/// If two buffers live in different regions or at different
-/// addresses, then they are disjoint.
+unfold
+let loc_addr_of_buffer (#t: Type) (b: buffer t) : GTot loc =
+  loc_addresses false (frameOf b) (Set.singleton (as_addr b))
 
-val as_addr_disjoint (#a1 #a2: Type) (b1: buffer a1) (b2: buffer a2) : Lemma
-  (requires (frameOf b1 <> frameOf b2 \/ as_addr b1 <> as_addr b2))
-  (ensures (disjoint b1 b2))
-  [SMTPatOr [
-    [SMTPat (disjoint b1 b2)];
-    [SMTPat (frameOf b1); SMTPat (frameOf b2)];
-    [SMTPat (as_addr b1); SMTPat (as_addr b2)];
-  ]]
+/// ``loc_regions r`` is the set of memory locations associated to a set
+/// ``r`` of regions.
+
+val loc_regions
+  (preserve_liveness: bool)
+  (r: Set.set HS.rid)
+: GTot loc
 
 
-/// The null pointer is disjoint from any buffer.
+/// ``loc_mreference b`` is the set of memory locations associated to a
+/// reference ``b``, which is actually the set of memory locations
+/// associated to the address of ``b``.
 
-val disjoint_null (a1: Type) (#a2: Type) (b2: buffer a2) : Lemma
-  (disjoint (null #a1) b2)
+unfold
+let loc_mreference
+  (#a: Type)
+  (#p: Preorder.preorder a)
+  (b: HS.mreference a p)
+: GTot loc
+= loc_addresses true (HS.frameOf b) (Set.singleton (HS.as_addr b))
 
-/// If two buffers span disjoint ranges from a common enclosing
-/// buffer, then they are disjoint.
+unfold
+let loc_freed_mreference
+  (#a: Type)
+  (#p: Preorder.preorder a)
+  (b: HS.mreference a p)
+: GTot loc
+= loc_addresses false (HS.frameOf b) (Set.singleton (HS.as_addr b))
 
-val gsub_disjoint (#a: Type) (b: buffer a) (i1 len1 i2 len2: U32.t) : Lemma
+
+/// ``loc_region_only r`` is the set of memory locations associated to a
+/// region ``r`` but not any region ``r'`` that extends ``r`` (in the sense
+/// of ``FStar.HyperStack.extends``.)
+
+unfold
+let loc_region_only
+  (preserve_liveness: bool)
+  (r: HS.rid)
+: GTot loc
+= loc_regions preserve_liveness (Set.singleton r)
+
+
+/// ``loc_all_regions_from r`` is the set of all memory locations
+/// associated to a region ``r`` and any region ``r'`` that transitively
+/// extends ``r`` (in the sense of ``FStar.HyperStack.extends``,
+/// e.g. nested stack frames.)
+
+unfold
+let loc_all_regions_from
+  (preserve_liveness: bool)
+  (r: HS.rid)
+: GTot loc
+= loc_regions preserve_liveness (HS.mod_set (Set.singleton r))
+
+
+/// We equip the ``loc`` monoid of sets of memory locations with an
+/// inclusion relation, ``loc_includes``, which is a preorder compatible
+/// with ``loc_union``. Although we consider sets of memory locations,
+/// we do not specify them using any F* set library such as
+/// ``FStar.Set``, ``FStar.TSet`` or ``FStar.GSet``, because ``loc_includes``
+/// encompasses more than just set-theoretic inclusion.
+
+val loc_includes
+  (s1 s2: loc)
+: GTot Type0
+
+val loc_includes_refl
+  (s: loc)
+: Lemma
+  (loc_includes s s)
+  [SMTPat (loc_includes s s)]
+
+val loc_includes_trans
+  (s1 s2 s3: loc)
+: Lemma
+  (requires (loc_includes s1 s2 /\ loc_includes s2 s3))
+  (ensures (loc_includes s1 s3))
+
+val loc_includes_union_r
+  (s s1 s2: loc)
+: Lemma
+  (requires (loc_includes s s1 /\ loc_includes s s2))
+  (ensures (loc_includes s (loc_union s1 s2)))
+  [SMTPat (loc_includes s (loc_union s1 s2))]
+
+val loc_includes_union_l
+  (s1 s2 s: loc)
+: Lemma
+  (requires (loc_includes s1 s \/ loc_includes s2 s))
+  (ensures (loc_includes (loc_union s1 s2) s))
+
+val loc_includes_none
+  (s: loc)
+: Lemma
+  (loc_includes s loc_none)
+  [SMTPat (loc_includes s loc_none)]
+
+
+/// If a buffer ``b1`` includes a buffer ``b2`` in the sense of the buffer
+/// theory (see ``LowStar.Buffer.includes``), then so are their
+/// corresponding sets of memory locations.
+
+val loc_includes_gsub_buffer_r
+  (l: loc)
+  (#t: Type)
+  (b: buffer t)
+  (i: UInt32.t)
+  (len: UInt32.t)
+: Lemma
+  (requires (UInt32.v i + UInt32.v len <= (length b) /\ loc_includes l (loc_buffer b)))
+  (ensures (UInt32.v i + UInt32.v len <= (length b) /\ loc_includes l (loc_buffer (gsub b i len))))
+  [SMTPat (loc_includes l (loc_buffer (gsub b i len)))]
+
+val loc_includes_gsub_buffer_l
+  (#t: Type)
+  (b: buffer t)
+  (i1: UInt32.t)
+  (len1: UInt32.t)
+  (i2: UInt32.t)
+  (len2: UInt32.t)
+: Lemma
+  (requires (UInt32.v i1 + UInt32.v len1 <= (length b) /\ UInt32.v i1 <= UInt32.v i2 /\ UInt32.v i2 + UInt32.v len2 <= UInt32.v i1 + UInt32.v len1))
+  (ensures (UInt32.v i1 + UInt32.v len1 <= (length b) /\ UInt32.v i1 <= UInt32.v i2 /\ UInt32.v i2 + UInt32.v len2 <= UInt32.v i1 + UInt32.v len1 /\ loc_includes (loc_buffer (gsub b i1 len1)) (loc_buffer (gsub b i2 len2))))
+  [SMTPat (loc_includes (loc_buffer (gsub b i1 len1)) (loc_buffer (gsub b i2 len2)))]
+
+/// If the contents of a buffer are equal in two given heaps, then so
+/// are the contents of any of its sub-buffers.
+
+val loc_includes_as_seq (#a: Type) (h1 h2: HS.mem) (larger smaller: buffer a) : Lemma
+  (requires (loc_includes (loc_buffer larger) (loc_buffer smaller) /\ as_seq h1 larger == as_seq h2 larger /\ (live h1 larger \/ live h1 smaller) /\ (live h2 larger \/ live h2 smaller)))
+  (ensures (as_seq h1 smaller == as_seq h2 smaller))
+
+
+/// Given a buffer ``b``, if its address is in a set ``s`` of addresses in
+/// the region of ``b``, then the set of memory locations corresponding
+/// to ``b`` is included in the set of memory locations corresponding to
+/// the addresses in ``s`` in region ``r``.
+///
+/// In particular, the set of memory locations corresponding to a
+/// buffer is included in the set of memory locations corresponding to
+/// its region and address.
+
+val loc_includes_addresses_buffer
+  (#t: Type)
+  (preserve_liveness: bool)
+  (r: HS.rid)
+  (s: Set.set nat)
+  (p: buffer t)
+: Lemma
+  (requires (frameOf p == r /\ Set.mem (as_addr p) s))
+  (ensures (loc_includes (loc_addresses preserve_liveness r s) (loc_buffer p)))
+  [SMTPat (loc_includes (loc_addresses preserve_liveness r s) (loc_buffer p))]
+
+
+/// The set of memory locations corresponding to a buffer is included
+/// in the set of memory locations corresponding to its region.
+
+val loc_includes_region_buffer
+  (#t: Type)
+  (preserve_liveness: bool)
+  (s: Set.set HS.rid)
+  (b: buffer t)
+: Lemma
+  (requires (Set.mem (frameOf b) s))
+  (ensures (loc_includes (loc_regions preserve_liveness s) (loc_buffer b)))
+  [SMTPat (loc_includes (loc_regions preserve_liveness s) (loc_buffer b))]
+
+
+/// If a region ``r`` is in a set of regions ``s``, then the set of memory
+/// locations corresponding to a set of addresses ``a`` in ``r`` is
+/// included in the set of memory locations corresponding to the
+/// regions in ``s``.
+///
+/// In particular, the the set of memory locations corresponding to a
+/// set of addresses ``a`` in a given region ``r`` is included in the set
+/// of memory locations corresponding to region ``r``.
+
+val loc_includes_region_addresses
+  (preserve_liveness1: bool)
+  (preserve_liveness2: bool)
+  (s: Set.set HS.rid)
+  (r: HS.rid)
+  (a: Set.set nat)
+: Lemma
+  (requires (Set.mem r s))
+  (ensures (loc_includes (loc_regions preserve_liveness1 s) (loc_addresses preserve_liveness2 r a)))
+  [SMTPat (loc_includes (loc_regions preserve_liveness1 s) (loc_addresses preserve_liveness2 r a))]
+
+/// If a set of region identifiers ``s1`` includes a set of region
+/// identifiers ``s2``, then so are their corresponding sets of memory
+/// locations.
+
+val loc_includes_region_region
+  (preserve_liveness1: bool)
+  (preserve_liveness2: bool)
+  (s1 s2: Set.set HS.rid)
+: Lemma
+  (requires ((preserve_liveness1 ==> preserve_liveness2) /\ Set.subset s2 s1))
+  (ensures (loc_includes (loc_regions preserve_liveness1 s1) (loc_regions preserve_liveness2 s2)))
+  [SMTPat (loc_includes (loc_regions preserve_liveness1 s1) (loc_regions preserve_liveness2 s2))]
+
+/// The following lemma can act as a cut when reasoning with sets of
+/// memory locations corresponding to sets of regions.
+
+val loc_includes_region_union_l
+  (preserve_liveness: bool)
+  (l: loc)
+  (s1 s2: Set.set HS.rid)
+: Lemma
+  (requires (loc_includes l (loc_regions preserve_liveness (Set.intersect s2 (Set.complement s1)))))
+  (ensures (loc_includes (loc_union (loc_regions preserve_liveness s1) l) (loc_regions preserve_liveness s2)))
+  [SMTPat (loc_includes (loc_union (loc_regions preserve_liveness s1) l) (loc_regions preserve_liveness s2))]
+
+
+/// If a set of addresses ``s1`` includes a set of addresses ``s2``,
+/// then so are their corresponding memory locations
+val loc_includes_addresses_addresses
+  (preserve_liveness1 preserve_liveness2: bool)
+  (r: HS.rid)
+  (s1 s2: Set.set nat)
+: Lemma
+  (requires ((preserve_liveness1 ==> preserve_liveness2) /\ Set.subset s2 s1))
+  (ensures (loc_includes (loc_addresses preserve_liveness1 r s1) (loc_addresses preserve_liveness2 r s2)))
+
+/// Patterns with loc_includes, union on the left
+
+let loc_includes_union_l_buffer
+  (s1 s2: loc)
+  (#t: Type)
+  (b: buffer t)
+: Lemma
+  (requires (loc_includes s1 (loc_buffer b) \/ loc_includes s2 (loc_buffer b)))
+  (ensures (loc_includes (loc_union s1 s2) (loc_buffer b)))
+  [SMTPat (loc_includes (loc_union s1 s2) (loc_buffer b))]
+= loc_includes_union_l s1 s2 (loc_buffer b)
+
+let loc_includes_union_l_addresses
+  (s1 s2: loc)
+  (prf: bool)
+  (r: HS.rid)
+  (a: Set.set nat)
+: Lemma
+  (requires (loc_includes s1 (loc_addresses prf r a) \/ loc_includes s2 (loc_addresses prf r a)))
+  (ensures (loc_includes (loc_union s1 s2) (loc_addresses prf r a)))
+  [SMTPat (loc_includes (loc_union s1 s2) (loc_addresses prf r a))]
+= loc_includes_union_l s1 s2 (loc_addresses prf r a)
+
+let loc_includes_union_l_regions
+  (s1 s2: loc)
+  (prf: bool)
+  (r: Set.set HS.rid)
+: Lemma
+  (requires (loc_includes s1 (loc_regions prf r) \/ loc_includes s2 (loc_regions prf r)))
+  (ensures (loc_includes (loc_union s1 s2) (loc_regions prf r)))
+  [SMTPat (loc_includes (loc_union s1 s2) (loc_regions prf r))]
+= loc_includes_union_l s1 s2 (loc_regions prf r)
+
+/// Since inclusion encompasses more than just set-theoretic
+/// inclusion, we also need to specify disjointness accordingly, as a
+/// symmetric relation compatible with union.
+
+val loc_disjoint
+  (s1 s2: loc)
+: GTot Type0
+
+val loc_disjoint_sym
+  (s1 s2: loc)
+: Lemma
+  (requires (loc_disjoint s1 s2))
+  (ensures (loc_disjoint s2 s1))
+
+let loc_disjoint_sym'
+  (s1 s2: loc)
+: Lemma
+  (loc_disjoint s1 s2 <==> loc_disjoint s2 s1)
+  [SMTPat (loc_disjoint s1 s2)]
+= Classical.move_requires (loc_disjoint_sym s1) s2;
+  Classical.move_requires (loc_disjoint_sym s2) s1
+
+val loc_disjoint_none_r
+  (s: loc)
+: Lemma
+  (ensures (loc_disjoint s loc_none))
+  [SMTPat (loc_disjoint s loc_none)]
+
+val loc_disjoint_union_r
+  (s s1 s2: loc)
+: Lemma
+  (requires (loc_disjoint s s1 /\ loc_disjoint s s2))
+  (ensures (loc_disjoint s (loc_union s1 s2)))
+
+
+/// If two sets of memory locations are disjoint, then so are any two
+/// included sets of memory locations.
+
+val loc_disjoint_includes
+  (p1 p2 p1' p2' : loc)
+: Lemma
+  (requires (loc_includes p1 p1' /\ loc_includes p2 p2' /\ loc_disjoint p1 p2))
+  (ensures (loc_disjoint p1' p2'))
+
+let loc_disjoint_union_r'
+  (s s1 s2: loc)
+: Lemma
+  (ensures (loc_disjoint s (loc_union s1 s2) <==> (loc_disjoint s s1 /\ loc_disjoint s s2)))
+  [SMTPat (loc_disjoint s (loc_union s1 s2))]
+= Classical.move_requires (loc_disjoint_union_r s s1) s2;
+  loc_includes_union_l s1 s2 s1;
+  loc_includes_union_l s1 s2 s2;
+  Classical.move_requires (loc_disjoint_includes s (loc_union s1 s2) s) s1;
+  Classical.move_requires (loc_disjoint_includes s (loc_union s1 s2) s) s2
+
+let loc_disjoint_includes_l (b1 b1' : loc) (b2: loc) : Lemma
+  (requires (loc_includes b1 b1' /\ loc_disjoint b1 b2))
+  (ensures (loc_disjoint b1' b2))
+  [SMTPat (loc_disjoint b1' b2); SMTPat (loc_includes b1 b1')]
+= loc_disjoint_includes b1 b2 b1' b2
+
+let loc_disjoint_includes_r (b1 : loc) (b2 b2': loc) : Lemma
+  (requires (loc_includes b2 b2' /\ loc_disjoint b1 b2))
+  (ensures (loc_disjoint b1 b2'))
+  [SMTPat (loc_disjoint b1 b2'); SMTPat (loc_includes b2 b2')]
+= loc_disjoint_includes b1 b2 b1 b2'
+
+
+val loc_disjoint_gsub_buffer
+  (#t: Type)
+  (b: buffer t)
+  (i1: UInt32.t)
+  (len1: UInt32.t)
+  (i2: UInt32.t)
+  (len2: UInt32.t)
+: Lemma
   (requires (
-    U32.v i1 + U32.v len1 <= length b /\
-    U32.v i2 + U32.v len2 <= length b /\
-    (U32.v i1 + U32.v len1 <= U32.v i2 \/ U32.v i2 + U32.v len2 <= U32.v i1)
+    UInt32.v i1 + UInt32.v len1 <= (length b) /\
+    UInt32.v i2 + UInt32.v len2 <= (length b) /\ (
+    UInt32.v i1 + UInt32.v len1 <= UInt32.v i2 \/
+    UInt32.v i2 + UInt32.v len2 <= UInt32.v i1
+  )))
+  (ensures (
+    UInt32.v i1 + UInt32.v len1 <= (length b) /\
+    UInt32.v i2 + UInt32.v len2 <= (length b) /\
+    loc_disjoint (loc_buffer (gsub b i1 len1)) (loc_buffer (gsub b i2 len2))
   ))
-  (ensures (disjoint (gsub b i1 len1) (gsub b i2 len2)))
-  [SMTPat (disjoint (gsub b i1 len1) (gsub b i2 len2))]
+  [SMTPat (loc_disjoint (loc_buffer (gsub b i1 len1)) (loc_buffer (gsub b i2 len2)))]
 
 
+/// If two sets of addresses correspond to different regions or are
+/// disjoint, then their corresponding sets of memory locations are
+/// disjoint.
+
+val loc_disjoint_addresses
+  (preserve_liveness1 preserve_liveness2: bool)
+  (r1 r2: HS.rid)
+  (n1 n2: Set.set nat)
+: Lemma
+  (requires (r1 <> r2 \/ Set.subset (Set.intersect n1 n2) Set.empty))
+  (ensures (loc_disjoint (loc_addresses preserve_liveness1 r1 n1) (loc_addresses preserve_liveness2 r2 n2)))
+  [SMTPat (loc_disjoint (loc_addresses preserve_liveness1 r1 n1) (loc_addresses preserve_liveness2 r2 n2))]
+
+/// If the region of a buffer ``p`` is not ``r``, or its address is not in
+/// the set ``n`` of addresses, then their corresponding sets of memory
+/// locations are disjoint.
+
+val loc_disjoint_buffer_addresses
+  (#t: Type)
+  (p: buffer t)
+  (preserve_liveness: bool)
+  (r: HS.rid)
+  (n: Set.set nat)
+: Lemma
+  (requires (r <> frameOf p \/ (~ (Set.mem (as_addr p) n))))
+  (ensures (loc_disjoint (loc_buffer p) (loc_addresses preserve_liveness r n)))
+  [SMTPat (loc_disjoint (loc_buffer p) (loc_addresses preserve_liveness r n))]
+
+val loc_disjoint_buffer_regions
+  (#t: Type)
+  (p: buffer t)
+  (preserve_liveness: bool)
+  (r: Set.set HS.rid)
+: Lemma
+  (requires (~ (frameOf p `Set.mem` r)))
+  (ensures (loc_disjoint (loc_buffer p) (loc_regions preserve_liveness r)))
+  [SMTPat (loc_disjoint (loc_buffer p) (loc_regions preserve_liveness r))]
+
+/// If two sets of region identifiers are disjoint, then so are their
+/// corresponding sets of memory locations.
+
+val loc_disjoint_regions
+  (preserve_liveness1: bool)
+  (preserve_liveness2: bool)
+  (rs1 rs2: Set.set HS.rid)
+: Lemma
+  (requires (Set.subset (Set.intersect rs1 rs2) Set.empty))
+  (ensures (loc_disjoint (loc_regions preserve_liveness1 rs1) (loc_regions preserve_liveness2 rs2)))
+  [SMTPat (loc_disjoint (loc_regions preserve_liveness1 rs1) (loc_regions preserve_liveness2 rs2))]
+
+
+/// The modifies clauses proper.
+///
+/// Let ``s`` be a set of memory locations, and ``h1`` and ``h2`` be two
+/// memory states. Then, ``s`` is modified from ``h1`` to ``h2`` only if,
+/// any memory location disjoint from ``s`` is preserved from ``h1`` into
+/// ``h2``. Elimination lemmas illustrating this principle follow.
+
+val modifies
+  (s: loc)
+  (h1 h2: HS.mem)
+: GTot Type0
+
+/// If a region ``r`` is disjoint from a set ``s`` of memory locations
+/// which is modified, then its liveness is preserved.
+
+val modifies_live_region
+  (s: loc)
+  (h1 h2: HS.mem)
+  (r: HS.rid)
+: Lemma
+  (requires (modifies s h1 h2 /\ loc_disjoint s (loc_region_only false r) /\ HS.live_region h1 r))
+  (ensures (HS.live_region h2 r))
+
+/// If a reference ``b`` is disjoint from a set ``p`` of memory locations
+/// which is modified, then its liveness and contents are preserved.
+
+val modifies_mreference_elim
+  (#t: Type)
+  (#pre: Preorder.preorder t)
+  (b: HS.mreference t pre)
+  (p: loc)
+  (h h': HS.mem)
+: Lemma
+  (requires (
+    loc_disjoint (loc_mreference b) p /\
+    HS.contains h b /\
+    modifies p h h'
+  ))
+  (ensures (
+    HS.contains h' b /\
+    HS.sel h b == HS.sel h' b
+  ))
+
+/// If a buffer ``b`` is disjoint from a set ``p`` of
+/// memory locations which is modified, then its liveness and contents
+/// are preserved.
+
+val modifies_buffer_elim
+  (#t1: Type)
+  (b: buffer t1)
+  (p: loc)
+  (h h': HS.mem)
+: Lemma
+  (requires (
+    loc_disjoint (loc_buffer b) p /\
+    live h b /\
+    modifies p h h'
+  ))
+  (ensures (
+    live h' b /\ (
+    as_seq h b == as_seq h' b
+  )))
+
+/// If the memory state does not change, then any memory location is
+/// modified (and, in particular, the empty set, ``loc_none``.)
+
+val modifies_refl
+  (s: loc)
+  (h: HS.mem)
+: Lemma
+  (modifies s h h)
+  [SMTPat (modifies s h h)]
+
+
+/// If a set ``s2`` of memory locations is modified, then so is any set
+/// ``s1`` that includes ``s2``. In other words, it is always possible to
+/// weaken a modifies clause by widening its set of memory locations.
+
+val modifies_loc_includes
+  (s1: loc)
+  (h h': HS.mem)
+  (s2: loc)
+: Lemma
+  (requires (modifies s2 h h' /\ loc_includes s1 s2))
+  (ensures (modifies s1 h h'))
+  [SMTPat (modifies s1 h h'); SMTPat (modifies s2 h h')]
+
+/// Some memory locations are tagged as liveness-insensitive: the
+/// liveness preservation of a memory location only depends on its
+/// disjointness from the liveness-sensitive memory locations of a
+/// modifies clause.
+
+val address_liveness_insensitive_locs: loc
+
+val region_liveness_insensitive_locs: loc
+
+val address_liveness_insensitive_buffer (#t: Type) (b: buffer t) : Lemma
+  (address_liveness_insensitive_locs `loc_includes` (loc_buffer b))
+  [SMTPat (address_liveness_insensitive_locs `loc_includes` (loc_buffer b))]
+
+val address_liveness_insensitive_addresses (r: HS.rid) (a: Set.set nat) : Lemma
+  (address_liveness_insensitive_locs `loc_includes` (loc_addresses true r a))
+  [SMTPat (address_liveness_insensitive_locs `loc_includes` (loc_addresses true r a))]
+
+val region_liveness_insensitive_buffer (#t: Type) (b: buffer t) : Lemma
+  (region_liveness_insensitive_locs `loc_includes` (loc_buffer b))
+  [SMTPat (region_liveness_insensitive_locs `loc_includes` (loc_buffer b))]
+
+val region_liveness_insensitive_addresses (preserve_liveness: bool) (r: HS.rid) (a: Set.set nat) : Lemma
+  (region_liveness_insensitive_locs `loc_includes` (loc_addresses preserve_liveness r a))
+  [SMTPat (region_liveness_insensitive_locs `loc_includes` (loc_addresses preserve_liveness r a))]
+
+val region_liveness_insensitive_regions (rs: Set.set HS.rid) : Lemma
+  (region_liveness_insensitive_locs `loc_includes` (loc_regions true rs))
+  [SMTPat (region_liveness_insensitive_locs `loc_includes` (loc_regions true rs))]
+
+val region_liveness_insensitive_address_liveness_insensitive:
+  squash (region_liveness_insensitive_locs `loc_includes` address_liveness_insensitive_locs)
+
+val modifies_liveness_insensitive_mreference
+  (l1 l2 : loc)
+  (h h' : HS.mem)
+  (#t: Type)
+  (#pre: Preorder.preorder t)
+  (x: HS.mreference t pre)
+: Lemma
+  (requires (modifies (loc_union l1 l2) h h' /\ loc_disjoint l1 (loc_mreference x) /\ address_liveness_insensitive_locs `loc_includes` l2 /\ h `HS.contains` x))
+  (ensures (h' `HS.contains` x))
+  (* TODO: pattern *)
+
+val modifies_liveness_insensitive_buffer
+  (l1 l2 : loc)
+  (h h' : HS.mem)
+  (#t: Type)
+  (x: buffer t)
+: Lemma
+  (requires (modifies (loc_union l1 l2) h h' /\ loc_disjoint l1 (loc_buffer x) /\ address_liveness_insensitive_locs `loc_includes` l2 /\ live h x))
+  (ensures (live h' x))
+  (* TODO: pattern *)
+
+let modifies_liveness_insensitive_mreference_weak
+  (l : loc)
+  (h h' : HS.mem)
+  (#t: Type)
+  (#pre: Preorder.preorder t)
+  (x: HS.mreference t pre)
+: Lemma
+  (requires (modifies l h h' /\ address_liveness_insensitive_locs `loc_includes` l /\ h `HS.contains` x))
+  (ensures (h' `HS.contains` x))
+= modifies_liveness_insensitive_mreference loc_none l h h' x
+
+let modifies_liveness_insensitive_buffer_weak
+  (l : loc)
+  (h h' : HS.mem)
+  (#t: Type)
+  (x: buffer t)
+: Lemma
+  (requires (modifies l h h' /\ address_liveness_insensitive_locs `loc_includes` l /\ live h x))
+  (ensures (live h' x))
+= modifies_liveness_insensitive_buffer loc_none l h h' x
+
+val modifies_liveness_insensitive_region
+  (l1 l2 : loc)
+  (h h' : HS.mem)
+  (x: HS.rid)
+: Lemma
+  (requires (modifies (loc_union l1 l2) h h' /\ loc_disjoint l1 (loc_region_only false x) /\ region_liveness_insensitive_locs `loc_includes` l2 /\ HS.live_region h x))
+  (ensures (HS.live_region h' x))
+  (* TODO: pattern *)
+
+val modifies_liveness_insensitive_region_mreference
+  (l1 l2 : loc)
+  (h h' : HS.mem)
+  (#t: Type)
+  (#pre: Preorder.preorder t)
+  (x: HS.mreference t pre)
+: Lemma
+  (requires (modifies (loc_union l1 l2) h h' /\ loc_disjoint l1 (loc_mreference x) /\ region_liveness_insensitive_locs `loc_includes` l2 /\ HS.live_region h (HS.frameOf x)))
+  (ensures (HS.live_region h' (HS.frameOf x)))
+  (* TODO: pattern *)
+
+val modifies_liveness_insensitive_region_buffer
+  (l1 l2 : loc)
+  (h h' : HS.mem)
+  (#t: Type)
+  (x: buffer t)
+: Lemma
+  (requires (modifies (loc_union l1 l2) h h' /\ loc_disjoint l1 (loc_buffer x) /\ region_liveness_insensitive_locs `loc_includes` l2 /\ HS.live_region h (frameOf x)))
+  (ensures (HS.live_region h' (frameOf x)))
+  (* TODO: pattern *)
+
+let modifies_liveness_insensitive_region_weak
+  (l2 : loc)
+  (h h' : HS.mem)
+  (x: HS.rid)
+: Lemma
+  (requires (modifies l2 h h' /\ region_liveness_insensitive_locs `loc_includes` l2 /\ HS.live_region h x))
+  (ensures (HS.live_region h' x))
+= modifies_liveness_insensitive_region loc_none l2 h h' x
+
+let modifies_liveness_insensitive_region_mreference_weak
+  (l2 : loc)
+  (h h' : HS.mem)
+  (#t: Type)
+  (#pre: Preorder.preorder t)
+  (x: HS.mreference t pre)
+: Lemma
+  (requires (modifies l2 h h' /\ region_liveness_insensitive_locs `loc_includes` l2 /\ HS.live_region h (HS.frameOf x)))
+  (ensures (HS.live_region h' (HS.frameOf x)))
+= modifies_liveness_insensitive_region_mreference loc_none l2 h h' x
+
+let modifies_liveness_insensitive_region_buffer_weak
+  (l2 : loc)
+  (h h' : HS.mem)
+  (#t: Type)
+  (x: buffer t)
+: Lemma
+  (requires (modifies l2 h h' /\ region_liveness_insensitive_locs `loc_includes` l2 /\ HS.live_region h (frameOf x)))
+  (ensures (HS.live_region h' (frameOf x)))
+= modifies_liveness_insensitive_region_buffer loc_none l2 h h' x
+
+
+/// Modifies clauses are transitive. This lemma is the most general
+/// one.
+
+val modifies_trans
+  (s12: loc)
+  (h1 h2: HS.mem)
+  (s23: loc)
+  (h3: HS.mem)
+: Lemma
+  (requires (modifies s12 h1 h2 /\ modifies s23 h2 h3))
+  (ensures (modifies (loc_union s12 s23) h1 h3))
+  [SMTPat (modifies s12 h1 h2); SMTPat (modifies s23 h2 h3)]
+
+/// Regions that are not live can be removed from sets of memory
+/// locations that are modified.
+
+val modifies_only_live_regions
+  (rs: Set.set HS.rid)
+  (l: loc)
+  (h h' : HS.mem)
+: Lemma
+  (requires (
+    modifies (loc_union (loc_regions false rs) l) h h' /\
+    (forall r . Set.mem r rs ==> (~ (HS.live_region h r)))
+  ))
+  (ensures (modifies l h h'))
+
+/// As a consequence, fresh regions can be removed from modifies
+/// clauses.
+
+val no_upd_fresh_region: r:HS.rid -> l:loc -> h0:HS.mem -> h1:HS.mem -> Lemma
+  (requires (HS.fresh_region r h0 h1 /\ modifies (loc_union (loc_all_regions_from false r) l) h0 h1))
+  (ensures  (modifies l h0 h1))
+  [SMTPat (HS.fresh_region r h0 h1); SMTPat (modifies l h0 h1)]
+
+val fresh_frame_modifies (h0 h1: HS.mem) : Lemma
+  (requires (HS.fresh_frame h0 h1))
+  (ensures (modifies loc_none h0 h1))
+
+val popped_modifies (h0 h1: HS.mem) : Lemma
+  (requires (HS.popped h0 h1))
+  (ensures (modifies (loc_region_only false (HS.get_tip h0)) h0 h1))
+
+/// Stack discipline: any stack frame (and all its transitively
+/// extending regions) that is pushed, modified and popped can be
+/// removed from a modifies clause.
+
+val modifies_fresh_frame_popped
+  (h0 h1: HS.mem)
+  (s: loc)
+  (h2 h3: HS.mem)
+: Lemma
+  (requires (
+    HS.fresh_frame h0 h1 /\
+    modifies (loc_union (loc_all_regions_from false (HS.get_tip h1)) s) h1 h2 /\
+    (HS.get_tip h2) == (HS.get_tip h1) /\
+    HS.popped h2 h3
+  ))
+  (ensures (
+    modifies s h0 h3 /\
+    (HS.get_tip h3) == HS.get_tip h0
+  ))
+  [SMTPat (HS.fresh_frame h0 h1); SMTPat (HS.popped h2 h3); SMTPat (modifies s h0 h3)]
+
+/// Compatibility lemmas to rescue modifies clauses specified in the
+/// standard F* HyperStack library.
+
+val modifies_loc_regions_intro
+  (rs: Set.set HS.rid)
+  (h1 h2: HS.mem)
+: Lemma
+  (requires (HS.modifies rs h1 h2))
+  (ensures (modifies (loc_regions true rs) h1 h2))
+
+val modifies_loc_addresses_intro
+  (r: HS.rid)
+  (a: Set.set nat)
+  (l: loc)
+  (h1 h2: HS.mem)
+: Lemma
+  (requires (
+    HS.live_region h2 r /\
+    modifies (loc_union (loc_region_only false r) l) h1 h2 /\
+    HS.modifies_ref r a h1 h2
+  ))
+  (ensures (modifies (loc_union (loc_addresses true r a) l) h1 h2))
+
+/// Modifies clauses for allocating a reference: nothing is
+/// modified. (In particular, a modifies clause does not track
+/// memory locations that are created.)
+
+val modifies_ralloc_post
+  (#a: Type)
+  (#rel: Preorder.preorder a)
+  (i: HS.rid)
+  (init: a)
+  (h: HS.mem)
+  (x: HST.mreference a rel { HST.is_eternal_region (HS.frameOf x) } )
+  (h' : HS.mem)
+: Lemma
+  (requires (HST.ralloc_post i init h x h'))
+  (ensures (modifies loc_none h h'))
+  [SMTPat (HST.ralloc_post i init h x h')]
+
+val modifies_salloc_post
+  (#a: Type)
+  (#rel: Preorder.preorder a)
+  (init: a)
+  (h: HS.mem)
+  (x: HST.mreference a rel { HS.is_stack_region (HS.frameOf x) } )
+  (h' : HS.mem)
+: Lemma
+  (requires (HST.salloc_post init h x h'))
+  (ensures (modifies loc_none h h'))
+  [SMTPat (HST.salloc_post init h x h')]
+
+/// Modifies clause for freeing a reference: the address is modified.
+
+val modifies_free
+  (#a: Type)
+  (#rel: Preorder.preorder a)
+  (r: HS.mreference a rel { HS.is_mm r } )
+  (m: HS.mem { m `HS.contains` r } )
+: Lemma
+  (modifies (loc_freed_mreference r) m (HS.free r m))
+  [SMTPat (HS.free r m)]
+
+/// Another compatibility lemma
+
+val modifies_none_modifies
+  (h1 h2: HS.mem)
+: Lemma
+  (requires (HST.modifies_none h1 h2))
+  (ensures (modifies loc_none h1 h2))
+  [SMTPat (HST.modifies_none h1 h2)]
+
+/// Compatibility with HS.upd
+
+val modifies_upd
+  (#t: Type) (#pre: Preorder.preorder t)
+  (r: HS.mreference t pre)
+  (v: t)
+  (h: HS.mem)
+: Lemma
+  (requires (HS.contains h r))
+  (ensures (modifies (loc_mreference r) h (HS.upd h r v)))
+  [SMTPat (HS.upd h r v)]
+
+///  A memory ``h`` does not contain address ``a`` in region ``r``, denoted
+///  ``does_not_contain_addr h (r, a)``, only if, either region ``r`` is
+///  not live, or address ``a`` is unused in region ``r``.
+
+(* BEGIN TODO: move to FStar.Monotonic.HyperStack *)
+
+val does_not_contain_addr
+  (h: HS.mem)
+  (ra: HS.rid * nat)
+: GTot Type0
+
+val not_live_region_does_not_contain_addr
+  (h: HS.mem)
+  (ra: HS.rid * nat)
+: Lemma
+  (requires (~ (HS.live_region h (fst ra))))
+  (ensures (h `does_not_contain_addr` ra))
+
+val unused_in_does_not_contain_addr
+  (h: HS.mem)
+  (#a: Type)
+  (#rel: Preorder.preorder a)
+  (r: HS.mreference a rel)
+: Lemma
+  (requires (r `HS.unused_in` h))
+  (ensures (h `does_not_contain_addr` (HS.frameOf r, HS.as_addr r)))
+
+val addr_unused_in_does_not_contain_addr
+  (h: HS.mem)
+  (ra: HS.rid * nat)
+: Lemma
+  (requires (HS.live_region h (fst ra) ==> snd ra `Heap.addr_unused_in` (Map.sel (HS.get_hmap h) (fst ra))))
+  (ensures (h `does_not_contain_addr` ra))
+
+val free_does_not_contain_addr
+  (#a: Type0)
+  (#rel: Preorder.preorder a)
+  (r: HS.mreference a rel)
+  (m: HS.mem)
+  (x: HS.rid * nat)
+: Lemma
+  (requires (
+    HS.is_mm r /\
+    m `HS.contains` r /\
+    fst x == HS.frameOf r /\
+    snd x == HS.as_addr r
+  ))
+  (ensures (
+    HS.free r m `does_not_contain_addr` x
+  ))
+  [SMTPat (HS.free r m `does_not_contain_addr` x)]
+
+val does_not_contain_addr_elim
+  (#a: Type0)
+  (#rel: Preorder.preorder a)
+  (r: HS.mreference a rel)
+  (m: HS.mem)
+  (x: HS.rid * nat)
+: Lemma
+  (requires (
+    m `does_not_contain_addr` x /\
+    HS.frameOf r == fst x /\
+    HS.as_addr r == snd x
+  ))
+  (ensures (~ (m `HS.contains` r)))
+
+(** END TODO *)
+
+/// Addresses that have not been allocated yet can be removed from
+/// modifies clauses.
+
+val modifies_only_live_addresses
+  (r: HS.rid)
+  (a: Set.set nat)
+  (l: loc)
+  (h h' : HS.mem)
+: Lemma
+  (requires (
+    modifies (loc_union (loc_addresses false r a) l) h h' /\
+    (forall x . Set.mem x a ==> h `does_not_contain_addr` (r, x))
+  ))
+  (ensures (modifies l h h'))
+
+
+(* Generic way to ensure that a buffer just allocated is disjoint from
+   any other object, however the latter's liveness is defined. *)
+
+val loc_not_unused_in (h: HS.mem) : GTot loc
+
+val loc_unused_in (h: HS.mem) : GTot loc
+
+val loc_unused_in_not_unused_in_disjoint (h: HS.mem) : Lemma
+  (loc_disjoint (loc_unused_in h) (loc_not_unused_in h))
+
+val live_loc_not_unused_in (#t: Type) (b: buffer t) (h: HS.mem) : Lemma
+  (requires (live h b))
+  (ensures (loc_not_unused_in h `loc_includes` loc_buffer b))
+  [SMTPat (live h b)]
+
+val unused_in_loc_unused_in (#t: Type) (b: buffer t) (h: HS.mem) : Lemma
+  (requires (unused_in b h))
+  (ensures (loc_unused_in h `loc_includes` loc_buffer b))
+  [SMTPat (unused_in b h)]
+
+val modifies_address_liveness_insensitive_unused_in
+  (h h' : HS.mem)
+: Lemma
+  (requires (modifies (address_liveness_insensitive_locs) h h'))
+  (ensures (loc_not_unused_in h' `loc_includes` loc_not_unused_in h /\ loc_unused_in h `loc_includes` loc_unused_in h'))
+
+val mreference_live_loc_not_unused_in
+  (#t: Type)
+  (#pre: Preorder.preorder t)
+  (h: HS.mem)
+  (r: HS.mreference t pre)
+: Lemma
+  (requires (h `HS.contains` r))
+  (ensures (loc_not_unused_in h `loc_includes` loc_freed_mreference r /\ loc_not_unused_in h `loc_includes` loc_mreference r))
+  [SMTPat (HS.contains h r)]
+
+val mreference_unused_in_loc_unused_in
+  (#t: Type)
+  (#pre: Preorder.preorder t)
+  (h: HS.mem)
+  (r: HS.mreference t pre)
+: Lemma
+  (requires (r `HS.unused_in` h))
+  (ensures (loc_unused_in h `loc_includes` loc_freed_mreference r /\ loc_unused_in h `loc_includes` loc_mreference r))
+  [SMTPat (HS.unused_in r h)]
+
+
+let unused_in_not_unused_in_disjoint_2
+  (l1 l2 l1' l2': loc)
+  (h: HS.mem)
+: Lemma
+  (requires (loc_unused_in h `loc_includes` l1 /\ loc_not_unused_in h `loc_includes` l2 /\ l1 `loc_includes` l1' /\ l2 `loc_includes` l2' ))
+  (ensures (loc_disjoint l1'  l2' ))
+  [SMTPat (loc_disjoint l1' l2'); SMTPat (loc_unused_in h `loc_includes` l1); SMTPat (loc_not_unused_in h `loc_includes` l2); SMTPat (l1 `loc_includes` l1') ; SMTPat (l2 `loc_includes` l2' )]
+= loc_includes_trans (loc_unused_in h) l1 l1' ;
+  loc_includes_trans (loc_not_unused_in h) l2 l2'  ;
+  loc_unused_in_not_unused_in_disjoint h ;
+  loc_disjoint_includes (loc_unused_in h) (loc_not_unused_in h) l1' l2' 
+
+let unused_in_not_unused_in_disjoint_1
+  (l1 l2 l1'  : loc)
+  (h: HS.mem)
+: Lemma
+  (requires (
+    loc_unused_in h `loc_includes` l1 /\
+    loc_not_unused_in h `loc_includes` l2 /\
+    l1 `loc_includes` l1' 
+  ))
+  (ensures (l1' `loc_disjoint` l2))
+  [SMTPat (loc_disjoint l1' l2); SMTPat (loc_unused_in h `loc_includes` l1); SMTPat (loc_not_unused_in h `loc_includes` l2)]
+= assert (loc_includes l2 l2)
+
+let unused_in_not_unused_in_disjoint_0
+  (l1 l2: loc)
+  (h: HS.mem)
+: Lemma
+  (requires (loc_unused_in h `loc_includes` l1 /\ loc_not_unused_in h `loc_includes` l2))
+  (ensures (loc_disjoint l1 l2))
+  [SMTPat (loc_disjoint l1 l2); SMTPat (loc_unused_in h `loc_includes` l1); SMTPat (loc_not_unused_in h `loc_includes` l2)]
+= assert (loc_includes l1 l1);
+  assert (loc_includes l2 l2)
+
+
+
+(* Duplicate the modifies clause to cope with cases that must not be used with transitivity *)
+
+abstract
+let modifies_inert
+  (s: loc)
+  (h1 h2: HS.mem)
+: GTot Type0
+= modifies s h1 h2
+
+abstract
+let modifies_inert_intro
+  (s: loc)
+  (h1 h2: HS.mem)
+: Lemma
+  (requires (modifies s h1 h2))
+  (ensures (modifies_inert s h1 h2))
+  [SMTPat (modifies s h1 h2)]
+= ()
+
+let modifies_inert_live_region
+  (s: loc)
+  (h1 h2: HS.mem)
+  (r: HS.rid)
+: Lemma
+  (requires (modifies_inert s h1 h2 /\ loc_disjoint s (loc_region_only false r) /\ HS.live_region h1 r))
+  (ensures (HS.live_region h2 r))
+  [SMTPatOr [
+    [SMTPat (modifies_inert s h1 h2); SMTPat (HS.live_region h1 r)];
+    [SMTPat (modifies_inert s h1 h2); SMTPat (HS.live_region h2 r)];
+  ]]
+= modifies_live_region s h1 h2 r
+
+let modifies_inert_mreference_elim
+  (#t: Type)
+  (#pre: Preorder.preorder t)
+  (b: HS.mreference t pre)
+  (p: loc)
+  (h h': HS.mem)
+: Lemma
+  (requires (
+    loc_disjoint (loc_mreference b) p /\
+    HS.contains h b /\
+    modifies_inert p h h'
+  ))
+  (ensures (
+    HS.contains h' b /\
+    HS.sel h b == HS.sel h' b
+  ))
+  [SMTPatOr [
+    [ SMTPat (modifies_inert p h h'); SMTPat (HS.sel h b) ] ;
+    [ SMTPat (modifies_inert p h h'); SMTPat (HS.contains h b) ];
+    [ SMTPat (modifies_inert p h h'); SMTPat (HS.sel h' b) ] ;
+    [ SMTPat (modifies_inert p h h'); SMTPat (HS.contains h' b) ]
+  ] ]
+= modifies_mreference_elim b p h h'
+
+let modifies_inert_buffer_elim
+  (#t1: Type)
+  (b: buffer t1)
+  (p: loc)
+  (h h': HS.mem)
+: Lemma
+  (requires (
+    loc_disjoint (loc_buffer b) p /\
+    live h b /\
+    modifies_inert p h h'
+  ))
+  (ensures (
+    live h' b /\ (
+    as_seq h b == as_seq h' b
+  )))
+  [SMTPatOr [
+    [ SMTPat (modifies_inert p h h'); SMTPat (as_seq h b) ] ;
+    [ SMTPat (modifies_inert p h h'); SMTPat (live h b) ];
+    [ SMTPat (modifies_inert p h h'); SMTPat (as_seq h' b) ] ;
+    [ SMTPat (modifies_inert p h h'); SMTPat (live h' b) ]
+  ] ]
+= modifies_buffer_elim b p h h'
+
+let modifies_inert_liveness_insensitive_mreference_weak
+  (l : loc)
+  (h h' : HS.mem)
+  (#t: Type)
+  (#pre: Preorder.preorder t)
+  (x: HS.mreference t pre)
+: Lemma
+  (requires (modifies_inert l h h' /\ address_liveness_insensitive_locs `loc_includes` l /\ h `HS.contains` x))
+  (ensures (h' `HS.contains` x))
+  [SMTPatOr [
+    [SMTPat (h `HS.contains` x); SMTPat (modifies_inert l h h');];
+    [SMTPat (h' `HS.contains` x); SMTPat (modifies_inert l h h');];
+  ]]
+= modifies_liveness_insensitive_mreference_weak l h h' x
+
+let modifies_inert_liveness_insensitive_buffer_weak
+  (l : loc)
+  (h h' : HS.mem)
+  (#t: Type)
+  (x: buffer t)
+: Lemma
+  (requires (modifies_inert l h h' /\ address_liveness_insensitive_locs `loc_includes` l /\ live h x))
+  (ensures (live h' x))
+  [SMTPatOr [
+    [SMTPat (live h x); SMTPat (modifies_inert l h h');];
+    [SMTPat (live h' x); SMTPat (modifies_inert l h h');];
+  ]]
+= modifies_liveness_insensitive_buffer_weak l h h' x
+
+let modifies_inert_liveness_insensitive_region_weak
+  (l2 : loc)
+  (h h' : HS.mem)
+  (x: HS.rid)
+: Lemma
+  (requires (modifies_inert l2 h h' /\ region_liveness_insensitive_locs `loc_includes` l2 /\ HS.live_region h x))
+  (ensures (HS.live_region h' x))
+  [SMTPatOr [
+    [SMTPat (modifies_inert l2 h h'); SMTPat (HS.live_region h x)];
+    [SMTPat (modifies_inert l2 h h'); SMTPat (HS.live_region h' x)];
+  ]]
+= modifies_liveness_insensitive_region_weak l2 h h' x
+
+let modifies_inert_liveness_insensitive_region_mreference_weak
+  (l2 : loc)
+  (h h' : HS.mem)
+  (#t: Type)
+  (#pre: Preorder.preorder t)
+  (x: HS.mreference t pre)
+: Lemma
+  (requires (modifies_inert l2 h h' /\ region_liveness_insensitive_locs `loc_includes` l2 /\ HS.live_region h (HS.frameOf x)))
+  (ensures (HS.live_region h' (HS.frameOf x)))
+  [SMTPatOr [
+    [SMTPat (modifies_inert l2 h h'); SMTPat (HS.live_region h (HS.frameOf x))];
+    [SMTPat (modifies_inert l2 h h'); SMTPat (HS.live_region h' (HS.frameOf x))];
+  ]]
+= modifies_liveness_insensitive_region_mreference_weak l2 h h' x
+
+let modifies_inert_liveness_insensitive_region_buffer_weak
+  (l2 : loc)
+  (h h' : HS.mem)
+  (#t: Type)
+  (x: buffer t)
+: Lemma
+  (requires (modifies_inert l2 h h' /\ region_liveness_insensitive_locs `loc_includes` l2 /\ HS.live_region h (frameOf x)))
+  (ensures (HS.live_region h' (frameOf x)))
+  [SMTPatOr [
+    [SMTPat (modifies_inert l2 h h'); SMTPat (HS.live_region h (frameOf x))];
+    [SMTPat (modifies_inert l2 h h'); SMTPat (HS.live_region h' (frameOf x))];
+  ]]
+= modifies_liveness_insensitive_region_buffer_weak l2 h h' x
+
+let fresh_frame_modifies_inert
+  (h0 h1: HS.mem)
+: Lemma
+  (requires (HS.fresh_frame h0 h1))
+  (ensures (modifies_inert loc_none h0 h1))
+  [SMTPat (HS.fresh_frame h0 h1)]
+= fresh_frame_modifies h0 h1
+
+let popped_modifies_inert
+  (h0 h1: HS.mem)
+: Lemma
+  (requires (HS.popped h0 h1))
+  (ensures (modifies_inert (loc_region_only false (HS.get_tip h0)) h0 h1))
+  [SMTPat (HS.popped h0 h1)]
+= popped_modifies h0 h1
+
+let modifies_inert_loc_unused_in
+  (l: loc)
+  (h1 h2: HS.mem)
+  (l' : loc)
+: Lemma
+  (requires (
+    modifies_inert l h1 h2 /\
+    address_liveness_insensitive_locs `loc_includes` l /\
+    loc_unused_in h2 `loc_includes` l'
+  ))
+  (ensures (loc_unused_in h1 `loc_includes` l'))
+  [SMTPat (modifies_inert l h1 h2); SMTPat (loc_unused_in h2 `loc_includes` l')]
+= modifies_loc_includes address_liveness_insensitive_locs h1 h2 l;
+  modifies_address_liveness_insensitive_unused_in h1 h2;
+  loc_includes_trans (loc_unused_in h1) (loc_unused_in h2) l'
+
+
+/// Legacy shorthands for disjointness and inclusion of buffers
+///
+let disjoint (#t1 #t2: Type) (b1: buffer t1) (b2: buffer t2) : GTot Type0 =
+  loc_disjoint (loc_buffer b1) (loc_buffer b2)
+
+let includes (#t: Type) (b1 b2: buffer t) : GTot Type0 =
+  loc_includes (loc_buffer b1) (loc_buffer b2) /\
+  (g_is_null b1 <==> g_is_null b2)
+
+val disjoint_neq (#a1 #a2: Type) (b1 : buffer a1) (b2 : buffer a2) : Lemma
+  (requires (disjoint b1 b2 /\ U32.v (len b1) > 0))
+  (ensures (~(b1 === b2)))
+
+/// The liveness of a sub-buffer is exactly equivalent to the liveness
+/// of its enclosing buffer.
+
+val includes_live (#a: Type) (h: HS.mem) (larger smaller: buffer a) : Lemma
+  (requires (larger `includes` smaller))
+  (ensures (live h larger <==> live h smaller))
+  [SMTPatOr [
+    [SMTPat (includes larger smaller); SMTPat (live h larger)];
+    [SMTPat (includes larger smaller); SMTPat (live h smaller)];
+  ]]
+
+val includes_frameOf_as_addr (#a: Type) (larger smaller: buffer a) : Lemma
+  (requires (larger `includes` smaller))
+  (ensures (g_is_null larger == g_is_null smaller /\ frameOf larger == frameOf smaller /\ as_addr larger == as_addr smaller))
+  [SMTPat (larger `includes` smaller)]
+/// 
 /// Useful shorthands for pointers, or maybe-null pointers
 
 inline_for_extraction
@@ -398,6 +1518,9 @@ inline_for_extraction
 type pointer_or_null (t: Type0) =
   b:buffer t { if g_is_null b then True else length b == 1 }
 
+unfold
+let deref #a (h: HS.mem) (x: pointer a) =
+  get h x 0
 
 /// Two pointers having different contents are disjoint. This is valid
 /// only for pointers, i.e. buffers of size 1.
@@ -416,239 +1539,6 @@ val pointer_distinct_sel_disjoint
   (ensures (
     disjoint b1 b2
   ))
-
-
-/// The following definitions are needed to implement the generic
-/// modifies clause. Those should not be used in client code. They
-/// appear in the interface only because the modifies clause is
-/// defined in another module, ``LowStar.Modifies``.
-
-val abuffer' (region: HS.rid) (addr: nat) : Tot Type0
-
-inline_for_extraction
-let abuffer (region: HS.rid) (addr: nat) : Tot Type0 = G.erased (abuffer' region addr)
-
-val abuffer_preserved (#r: HS.rid) (#a: nat) (b: abuffer r a) (h h' : HS.mem) : GTot Type0
-
-val abuffer_preserved_refl (#r: HS.rid) (#a: nat) (b: abuffer r a) (h : HS.mem) : Lemma
-  (abuffer_preserved b h h)
-
-val abuffer_preserved_trans (#r: HS.rid) (#a: nat) (b: abuffer r a) (h1 h2 h3 : HS.mem) : Lemma
-  (requires (abuffer_preserved b h1 h2 /\ abuffer_preserved b h2 h3))
-  (ensures (abuffer_preserved b h1 h3))
-
-val same_mreference_abuffer_preserved
-  (#r: HS.rid)
-  (#a: nat)
-  (b: abuffer r a)
-  (h1 h2: HS.mem)
-  (f: (
-    (a' : Type) ->
-    (pre: Preorder.preorder a') ->
-    (r': HS.mreference a' pre) ->
-    Lemma
-    (requires (h1 `HS.contains` r' /\ r == HS.frameOf r' /\ a == HS.as_addr r'))
-    (ensures (h2 `HS.contains` r' /\ h1 `HS.sel` r' == h2 `HS.sel` r'))
-  ))
-: Lemma
-  (abuffer_preserved b h1 h2)
-
-val addr_unused_in_abuffer_preserved
-  (#r: HS.rid)
-  (#a: nat)
-  (b: abuffer r a)
-  (h1 h2: HS.mem)
-: Lemma
-  (requires (HS.live_region h1 r ==> a `Heap.addr_unused_in` (Map.sel (HS.get_hmap h1) r)))
-  (ensures (abuffer_preserved b h1 h2))
-
-val abuffer_of_buffer (#t: Type) (b: buffer t) : Tot (abuffer (frameOf b) (as_addr b))
-
-val abuffer_preserved_elim (#t: Type) (b: buffer t) (h h' : HS.mem) : Lemma
-  (requires (abuffer_preserved #(frameOf b) #(as_addr b) (abuffer_of_buffer b) h h' /\ live h b))
-  (ensures (live h' b /\ as_seq h b == as_seq h' b))
-
-let unused_in_abuffer_preserved
-  (#t: Type)
-  (b: buffer t)
-  (h h' : HS.mem)
-: Lemma
-  (requires (b `unused_in` h))
-  (ensures (abuffer_preserved #(frameOf b) #(as_addr b) (abuffer_of_buffer b) h h'))
-= Classical.move_requires (fun b -> live_not_unused_in #t h b) b;
-  live_null t h;
-  null_unique b;
-  unused_in_equiv b h;
-  addr_unused_in_abuffer_preserved #(frameOf b) #(as_addr b) (abuffer_of_buffer b) h h'
-
-val abuffer_includes (#r: HS.rid) (#a: nat) (larger smaller: abuffer r a) : GTot Type0
-
-val abuffer_includes_refl (#r: HS.rid) (#a: nat) (b: abuffer r a) : Lemma
-  (b `abuffer_includes` b)
-
-val abuffer_includes_trans (#r: HS.rid) (#a: nat) (b1 b2 b3: abuffer r a) : Lemma
-  (requires (b1 `abuffer_includes` b2 /\ b2 `abuffer_includes` b3))
-  (ensures (b1 `abuffer_includes` b3))
-
-val abuffer_includes_abuffer_preserved (#r: HS.rid) (#a: nat) (larger smaller: abuffer r a) (h1 h2: HS.mem) : Lemma
-  (requires (larger `abuffer_includes` smaller /\ abuffer_preserved larger h1 h2))
-  (ensures (abuffer_preserved smaller h1 h2))
-
-val abuffer_includes_intro (#t: Type) (larger smaller: buffer t) : Lemma
-  (requires (larger `includes` smaller))
-  (ensures (
-    let r = frameOf larger in
-    let a = as_addr larger in
-    abuffer_includes #r #a (abuffer_of_buffer larger) (abuffer_of_buffer smaller)
-  ))
-
-val abuffer_disjoint (#r: HS.rid) (#a: nat) (b1 b2: abuffer r a) : GTot Type0
-
-val abuffer_disjoint_sym (#r: HS.rid) (#a: nat) (b1 b2: abuffer r a) : Lemma
-  (abuffer_disjoint b1 b2 <==> abuffer_disjoint b2 b1)
-
-val abuffer_disjoint_includes (#r: HS.rid) (#a: nat) (larger1 larger2: abuffer r a) (smaller1 smaller2: abuffer r a) : Lemma
-  (requires (abuffer_disjoint larger1 larger2 /\ larger1 `abuffer_includes` smaller1 /\ larger2 `abuffer_includes` smaller2))
-  (ensures (abuffer_disjoint smaller1 smaller2))
-
-val abuffer_disjoint_intro (#t1 #t2: Type) (b1: buffer t1) (b2: buffer t2) : Lemma
-  (requires (disjoint b1 b2 /\ frameOf b1 == frameOf b2 /\ as_addr b1 == as_addr b2))
-  (ensures (
-    let r = frameOf b1 in
-    let a = as_addr b1 in
-    abuffer_disjoint #r #a (abuffer_of_buffer b1) (abuffer_of_buffer b2)
-  ))
-
-val liveness_preservation_intro
-  (#t: Type) (h h' : HS.mem) (b: buffer t)
-  (f: (
-    (t' : Type) ->
-    (pre: Preorder.preorder t') ->
-    (r: HS.mreference t' pre) ->
-    Lemma
-    (requires (HS.frameOf r == frameOf b /\ HS.as_addr r == as_addr b /\ h `HS.contains` r))
-    (ensures (h' `HS.contains` r))
-  ))
-: Lemma
-  (requires (live h b))
-  (ensures (live h' b))
-
-(* Basic, non-compositional modifies clauses, used only to implement the generic modifies clause. DO NOT USE in client code *)
-
-val modifies_0 (h1 h2: HS.mem) : GTot Type0
-
-val modifies_0_live_region (h1 h2: HS.mem) (r: HS.rid) : Lemma
-  (requires (modifies_0 h1 h2 /\ HS.live_region h1 r))
-  (ensures (HS.live_region h2 r))
-
-val modifies_0_mreference (#a: Type) (#pre: Preorder.preorder a) (h1 h2: HS.mem) (r: HS.mreference a pre) : Lemma
-  (requires (modifies_0 h1 h2 /\ h1 `HS.contains` r))
-  (ensures (h2 `HS.contains` r /\ h1 `HS.sel` r == h2 `HS.sel` r))
-
-let modifies_0_abuffer
-  (#r: HS.rid)
-  (#a: nat)
-  (b: abuffer r a)
-  (h1 h2: HS.mem)
-: Lemma
-  (requires (modifies_0 h1 h2))
-  (ensures (abuffer_preserved b h1 h2))
-= same_mreference_abuffer_preserved b h1 h2 (fun a' pre r' -> modifies_0_mreference h1 h2 r')
-
-val modifies_0_unused_in
-  (h1 h2: HS.mem)
-  (r: HS.rid)
-  (n: nat)
-: Lemma
-  (requires (
-    modifies_0 h1 h2 /\
-    HS.live_region h1 r /\ HS.live_region h2 r /\
-    n `Heap.addr_unused_in` (HS.get_hmap h2 `Map.sel` r)
-  ))
-  (ensures (n `Heap.addr_unused_in` (HS.get_hmap h1 `Map.sel` r)))
-
-val modifies_1 (#a: Type) (b: buffer a) (h1 h2: HS.mem) : GTot Type0
-
-val modifies_1_live_region (#a: Type) (b: buffer a) (h1 h2: HS.mem) (r: HS.rid) : Lemma
-  (requires (modifies_1 b h1 h2 /\ HS.live_region h1 r))
-  (ensures (HS.live_region h2 r))
-
-val modifies_1_liveness
-  (#a: Type) (b: buffer a) (h1 h2: HS.mem)
-  (#a': Type) (#pre: Preorder.preorder a') (r' : HS.mreference a' pre)
-: Lemma
-  (requires (modifies_1 b h1 h2 /\ h1 `HS.contains` r'))
-  (ensures (h2 `HS.contains` r'))
-
-val modifies_1_unused_in
-  (#t: Type)
-  (b: buffer t)
-  (h1 h2: HS.mem)
-  (r: HS.rid)
-  (n: nat)
-: Lemma
-  (requires (
-    modifies_1 b h1 h2 /\
-    HS.live_region h1 r /\ HS.live_region h2 r /\
-    n `Heap.addr_unused_in` (HS.get_hmap h2 `Map.sel` r)
-  ))
-  (ensures (n `Heap.addr_unused_in` (HS.get_hmap h1 `Map.sel` r)))
-
-val modifies_1_mreference
-  (#a: Type) (b: buffer a)
-  (h1 h2: HS.mem)
-  (#a': Type) (#pre: Preorder.preorder a') (r' : HS.mreference a' pre)
-: Lemma
-  (requires (modifies_1 b h1 h2 /\ (frameOf b <> HS.frameOf r' \/ as_addr b <> HS.as_addr r') /\ h1 `HS.contains` r'))
-  (ensures (h2 `HS.contains` r' /\ h1 `HS.sel` r' == h2 `HS.sel` r'))
-
-val modifies_1_abuffer
-  (#a: Type) (b : buffer a)
-  (h1 h2: HS.mem)
-  (b' : abuffer (frameOf b) (as_addr b))
-: Lemma
-  (requires (modifies_1 b h1 h2 /\ abuffer_disjoint #(frameOf b) #(as_addr b) (abuffer_of_buffer b) b'))
-  (ensures (abuffer_preserved #(frameOf b) #(as_addr b) b' h1 h2))
-
-val modifies_1_null
-  (#a: Type) (b: buffer a)
-  (h1 h2: HS.mem)
-: Lemma
-  (requires (modifies_1 b h1 h2 /\ g_is_null b))
-  (ensures (modifies_0 h1 h2))
-
-val modifies_addr_of
-  (#a: Type)
-  (b: buffer a)
-  (h1 h2: HS.mem)
-: GTot Type0
-
-val modifies_addr_of_live_region (#a: Type) (b: buffer a) (h1 h2: HS.mem) (r: HS.rid) : Lemma
-  (requires (modifies_addr_of b h1 h2 /\ HS.live_region h1 r))
-  (ensures (HS.live_region h2 r))
-
-val modifies_addr_of_mreference
-  (#a: Type) (b: buffer a)
-  (h1 h2: HS.mem)
-  (#a': Type) (#pre: Preorder.preorder a') (r' : HS.mreference a' pre)
-: Lemma
-  (requires (modifies_addr_of b h1 h2 /\ (frameOf b <> HS.frameOf r' \/ as_addr b <> HS.as_addr r') /\ h1 `HS.contains` r'))
-  (ensures (h2 `HS.contains` r' /\ h1 `HS.sel` r' == h2 `HS.sel` r'))
-
-val modifies_addr_of_unused_in
-  (#t: Type)
-  (b: buffer t)
-  (h1 h2: HS.mem)
-  (r: HS.rid)
-  (n: nat)
-: Lemma
-  (requires (
-    modifies_addr_of b h1 h2 /\
-    (r <> frameOf b \/ n <> as_addr b) /\
-    HS.live_region h1 r /\ HS.live_region h2 r /\
-    n `Heap.addr_unused_in` (HS.get_hmap h2 `Map.sel` r)
-  ))
-  (ensures (n `Heap.addr_unused_in` (HS.get_hmap h1 `Map.sel` r)))
 
 
 /// The following stateful operations on buffers do not change the
@@ -682,6 +1572,7 @@ val sub (#a: Type) (b: buffer a) (i: U32.t) (len: U32.t) : HST.Stack (buffer a)
 val offset (#a: Type) (b: buffer a) (i: U32.t) : HST.Stack (buffer a)
   (requires (fun h -> U32.v i <= length b /\ live h b))
   (ensures (fun h y h' -> h == h' /\ y == gsub b i (U32.sub (len b) i)))
+// goffset
 
 
 /// ``index b i`` reads the value of ``b`` at offset ``i`` from memory and
@@ -693,15 +1584,6 @@ val index (#a: Type) (b: buffer a) (i: U32.t) : HST.Stack a
 
 /// The following stateful operations on buffers modify the memory,
 /// and, as usual, require the liveness of the buffer.
-
-(* FIXME: their postconditions are using non-compositional modifies
-   clauses, which are automatically converted to compositional
-   modifies clauses by lemmas from LowStar.Modifies through
-   patterns. In a future version, LowStar.Modifies could actually be
-   merged into LowStar.Buffers so that postconditions of those
-   operations would directly be specified in terms of the
-   compositional modifies clauses.
- *)
 
 /// ``g_upd_seq b s h`` updates the entire buffer `b`'s contents in
 /// heap `h` to correspond to the sequence `s`
@@ -718,7 +1600,7 @@ val g_upd_seq_as_seq (#a:Type)
                      (s:Seq.lseq a (length b))
                      (h:HS.mem{live h b})
   : Lemma (let h' = g_upd_seq b s h in
-           modifies_1 b h h' /\
+           modifies (loc_buffer b) h h' /\
            live h' b /\
            as_seq h' b == s)
 
@@ -744,7 +1626,7 @@ val upd
   (requires (fun h -> live h b /\ U32.v i < length b))
   (ensures (fun h _ h' ->
     (not (g_is_null b)) /\
-    modifies_1 b h h' /\
+    modifies (loc_buffer b) h h' /\
     live h' b /\
     as_seq h' b == Seq.upd (as_seq h b) (U32.v i) v
   ))
@@ -783,7 +1665,7 @@ val free
     (not (g_is_null b)) /\
     Map.domain (HS.get_hmap h1) `Set.equal` Map.domain (HS.get_hmap h0) /\ 
     (HS.get_tip h1) == (HS.get_tip h0) /\
-    modifies_addr_of b h0 h1 /\
+    modifies (loc_addr_of_buffer b) h0 h1 /\
     HS.live_region h1 (frameOf b)
   ))
 
@@ -815,7 +1697,7 @@ let alloc_post_common
   live h1 b /\
   Map.domain (HS.get_hmap h1) `Set.equal` Map.domain (HS.get_hmap h0) /\ 
   (HS.get_tip h1) == (HS.get_tip h0) /\
-  modifies_0 h0 h1
+  modifies loc_none h0 h1
 
 /// ``gcmalloc r init len`` allocates a memory-managed buffer of some
 /// positive length ``len`` in an eternal region ``r``. Every cell of this
@@ -917,3 +1799,132 @@ val gcmalloc_of_list
     alloc_post_common r len b h h' /\
     as_seq h' b == Seq.of_list init
   ))
+
+/// Derived operations
+
+#set-options "--z3rlimit 16" // necessary here because of interleaving blit with the .fst file
+
+let rec blit
+  (#t: Type)
+  (src: buffer t)
+  (idx_src: U32.t)
+  (dst: buffer t)
+  (idx_dst: U32.t)
+  (len: U32.t)
+: HST.Stack unit
+  (requires (fun h ->
+    live h src /\ live h dst /\ disjoint src dst /\
+    U32.v idx_src + U32.v len <= length src /\
+    U32.v idx_dst + U32.v len <= length dst
+  ))
+  (ensures (fun h _ h' ->
+    modifies (loc_buffer dst) h h' /\
+    live h' dst /\
+    Seq.slice (as_seq h' dst) (U32.v idx_dst) (U32.v idx_dst + U32.v len) ==
+    Seq.slice (as_seq h src) (U32.v idx_src) (U32.v idx_src + U32.v len) /\
+    Seq.slice (as_seq h' dst) 0 (U32.v idx_dst) ==
+    Seq.slice (as_seq h dst) 0 (U32.v idx_dst) /\
+    Seq.slice (as_seq h' dst) (U32.v idx_dst + U32.v len) (length dst) ==
+    Seq.slice (as_seq h dst) (U32.v idx_dst + U32.v len) (length dst)
+  ))
+= let h0 = HST.get () in
+  if len = 0ul then ()
+  else begin
+    let len' = U32.(len -^ 1ul) in
+    blit #t src idx_src dst idx_dst len';
+    let z = U32.(index src (idx_src +^ len')) in
+    upd dst (U32.(idx_dst +^ len')) z;
+    let h1 = HST.get() in
+    Seq.snoc_slice_index (as_seq h1 dst) (U32.v idx_dst) (U32.v idx_dst + U32.v len');
+    Seq.cons_head_tail (Seq.slice (as_seq h0 dst) (U32.v idx_dst + U32.v len') (length dst));
+    Seq.cons_head_tail (Seq.slice (as_seq h1 dst) (U32.v idx_dst + U32.v len') (length dst))
+  end
+
+#set-options "--z3rlimit 16" // necessary here because of assign_list in the .fsti itself
+
+module L = FStar.List.Tot
+
+inline_for_extraction
+let rec assign_list #a (l: list a) (b: buffer a): HST.Stack unit
+  (requires (fun h0 ->
+    live h0 b /\
+    length b = L.length l))
+  (ensures (fun h0 _ h1 ->
+    live h1 b /\
+    (modifies (loc_buffer b) h0 h1) /\
+    as_seq h1 b == Seq.seq_of_list l))
+=
+  match l with
+  | [] -> 
+      let h = HST.get () in
+      assert (length b = 0);
+      assert (Seq.length (as_seq h b) = 0);
+      assert (Seq.equal (as_seq h b) (Seq.empty #a));
+      assert (Seq.seq_of_list [] `Seq.equal` Seq.empty #a)
+  | hd :: tl ->
+      let b_hd = sub b 0ul 1ul in
+      let b_tl = offset b 1ul in
+      let h = HST.get () in
+      upd b_hd 0ul hd;
+      let h0 = HST.get () in
+      assign_list tl b_tl;
+      let h1 = HST.get () in
+      assert (as_seq h1 b_hd == as_seq h0 b_hd);
+      assert (get h1 b_hd 0 == hd);
+      assert (as_seq h1 b_tl == Seq.seq_of_list tl);
+      assert (Seq.equal (as_seq h1 b) (Seq.append (as_seq h1 b_hd) (as_seq h1 b_tl)));
+      assert ((Seq.seq_of_list l) == (Seq.cons hd (Seq.seq_of_list tl)))
+
+#reset-options
+
+
+/// Type class instantiation for compositionality with other kinds of memory locations than regions, references or buffers (just in case).
+/// No usage pattern has been found yet.
+
+module MG = FStar.ModifiesGen
+
+val abuffer' (region: HS.rid) (addr: nat) : Tot Type0
+
+inline_for_extraction
+let abuffer (region: HS.rid) (addr: nat) : Tot Type0 = G.erased (abuffer' region addr)
+
+val cloc_cls: MG.cls abuffer
+
+val cloc_of_loc (l: loc) : Tot (MG.loc cloc_cls)
+
+val loc_of_cloc (l: MG.loc cloc_cls) : Tot loc
+
+val loc_of_cloc_of_loc (l: loc) : Lemma
+  (loc_of_cloc (cloc_of_loc l) == l)
+  [SMTPat (loc_of_cloc (cloc_of_loc l))]
+
+val cloc_of_loc_of_cloc (l: MG.loc cloc_cls) : Lemma
+  (cloc_of_loc (loc_of_cloc l) == l)
+  [SMTPat (cloc_of_loc (loc_of_cloc l))]
+
+val cloc_of_loc_none: unit -> Lemma (cloc_of_loc loc_none == MG.loc_none)
+
+val cloc_of_loc_union (l1 l2: loc) : Lemma
+  (cloc_of_loc (loc_union l1 l2) == MG.loc_union (cloc_of_loc l1) (cloc_of_loc l2))
+
+val cloc_of_loc_addresses
+  (preserve_liveness: bool)
+  (r: HS.rid)
+  (n: Set.set nat)
+: Lemma
+  (cloc_of_loc (loc_addresses preserve_liveness r n) == MG.loc_addresses preserve_liveness r n)
+
+val cloc_of_loc_regions
+  (preserve_liveness: bool)
+  (r: Set.set HS.rid)
+: Lemma
+  (cloc_of_loc (loc_regions preserve_liveness r) == MG.loc_regions preserve_liveness r)
+
+val loc_includes_to_cloc (l1 l2: loc) : Lemma
+  (loc_includes l1 l2 <==> MG.loc_includes (cloc_of_loc l1) (cloc_of_loc l2))
+
+val loc_disjoint_to_cloc (l1 l2: loc) : Lemma
+  (loc_disjoint l1 l2 <==> MG.loc_disjoint (cloc_of_loc l1) (cloc_of_loc l2))
+
+val modifies_to_cloc (l: loc) (h1 h2: HS.mem) : Lemma
+  (modifies l h1 h2 <==> MG.modifies (cloc_of_loc l) h1 h2)
