ulib/LowStar.BufferCompat.fst
@@ -26,7 +26,7 @@ let rfree
     (not (g_is_null b)) /\
     Map.domain (HS.get_hmap h1) `Set.equal` Map.domain (HS.get_hmap h0) /\ 
     (HS.get_tip h1) == (HS.get_tip h0) /\
-    modifies_addr_of b h0 h1 /\
+    modifies (loc_addr_of_buffer b) h0 h1 /\
     HS.live_region h1 (frameOf b)
   ))
 = free b
